Reproved FactorialRecur.v with the new program logic

platform/cito/examples/FactorialRecur.v
@@ -17,10 +17,6 @@ Definition fact_w (w : W) := natToW (fact (wordToNat w)).
 Definition body := (
   If (0 < "n") {
     "ret" <-- DCall "fact"!"fact" ("n" - 1);;
-    (* Assert [ *)
-    (*   BEFORE(V, h) *)
-    (*   AFTER(V', h') *)
-    (*   V' "ret" = fact_w (V "n" ^- $1) /\ h' = h ];; *)
     "ret" <- "n" * "ret"
   } else {
     "ret" <- 1
@@ -91,149 +87,133 @@ Definition fact_spec : ForeignFuncSpec :=
                                           /\ ret = inl (fact_w n)
   |}.
 
+Definition specs := add ("fact", "fact") (Foreign fact_spec) (empty _).
+
 Definition change_fs (fs : settings -> W -> option Callee) : settings -> W -> option Callee := 
   fun stn w =>
     match fs stn w with
-      | None => None
-      | Some _ => Some (Foreign fact_spec)
+      | Some (Semantics.Internal _) => Some (Foreign fact_spec)
+      | other => other
     end.
 
-Definition fs_good_to_use' specs (fs : settings -> W -> option Callee) (stn : settings) :=
-  forall p spec, 
-    fs stn p = Some spec <-> 
-    exists lbl : glabel,
-      Labels stn lbl = Some p /\
-      find lbl specs = Some spec.
-
-Definition specs := add ("fact", "fact") (Foreign fact_spec) (empty _).
-
-Definition dummy_gf : GoodFunction.
-  refine (to_good_function f _).
-  good_module.
-Defined.    
-
-Definition spec_op := hd dummy_gf (Functions gm).
-
-Definition specs_op := add ("fact", "fact") (Internal spec_op) (empty _).
-
-Lemma fs_good : forall fs stn, fs_good_to_use modules imports fs stn -> fs_good_to_use' specs_op fs stn.
-  unfold modules, imports.
+Lemma change_fs_agree : forall fs stn, stn_good_to_use modules imports stn -> fs_good_to_use modules imports fs stn -> specs_env_agree specs (from_bedrock_label_map (Labels stn), change_fs fs stn).
   intros.
-  unfold fs_good_to_use, fs_good_to_use' in *.
-  split; intros.
-  eapply H in H0.
-  openhyp.
-  subst.
-  descend; eauto.
-  unfold specs_op.
-  eapply find_mapsto_iff.
-  eapply add_mapsto_iff.
-  left.
-  unfold spec_op, gm, to_good_module in *; simpl in *.
-  openhyp.
-  subst; simpl in *.
-  openhyp.
-  subst; simpl in *.
-  eauto.
-  intuition.
-  intuition.
-  rewrite empty_o in H2; intuition.
-  openhyp.
-  unfold specs_op in *.
-  eapply find_mapsto_iff in H1.
-  eapply add_mapsto_iff in H1.
-  openhyp.
-  subst.
+  split.
+  simpl.
+  unfold labels_in_scope.
+  intros.
   eapply H.
-  descend; eauto.
+  unfold specs in *.
+  eapply add_in_iff in H1.
+  openhyp.
+  subst; simpl in *.
   left.
-  descend; eauto.
-  unfold spec_op, gm, to_good_module; simpl; eauto.
-  eapply empty_mapsto_iff in H2; intuition.
-Qed.
+  unfold gm, to_good_module in *; simpl in *.
+  descend.
+  eauto.
+  simpl; eauto.
+  simpl; eauto.
+  eapply empty_in_iff in H1; intuition.
 
-Lemma change_fs_good : forall fs stn, fs_good_to_use modules imports fs stn -> fs_good_to_use' specs (change_fs fs) stn.
-  unfold modules, imports.
+  unfold specs_fs_agree; simpl in *.
+  unfold change_fs.
   intros.
-  eapply fs_good in H.
-  unfold fs_good_to_use', change_fs in *.
-  split; intros.
   destruct (option_dec (fs0 stn p)).
   destruct s; rewrite e in *.
-  injection H0; intros; subst.
-  eapply H in e.
+  destruct x; simpl in *.
+  eapply H0 in e.
   openhyp.
-  unfold specs_op in *.
+  subst; simpl in *.
+  openhyp.
+  subst; simpl in *.
+  openhyp.
+  subst; simpl in *.
+  discriminate.
+  intuition.
+  intuition.
+  injection H2; intros; subst.
+  unfold imports in H3; simpl in *.
+  compute in H3; intuition.
+  split; intros.
+  injection H1; intros; subst.
+  eapply H0 in e.
+  openhyp.
+  subst; simpl in *.
+  openhyp.
+  subst; simpl in *.
+  openhyp.
+  subst; simpl in *.
+  injection H3; intros; subst; simpl in *; clear H3.
+  descend.
+  eauto.
+  reflexivity.
+  intuition.
+  intuition.
+  compute in H4; intuition.
+  openhyp.
+  unfold specs in H2.
   eapply find_mapsto_iff in H2.
   eapply add_mapsto_iff in H2.
   openhyp.
-  subst.
-  descend; eauto.
+  subst; eauto.
   eapply empty_mapsto_iff in H3; intuition.
-  rewrite e in *; intuition.
+  rewrite e in *.
+  split; intros.
+  discriminate.
   openhyp.
-  unfold specs in *.
-  eapply find_mapsto_iff in H1.
-  eapply add_mapsto_iff in H1.
+  unfold specs in H2.
+  eapply find_mapsto_iff in H2.
+  eapply add_mapsto_iff in H2.
   openhyp.
-  subst.
-  assert (fs0 stn p = Some (Internal spec_op)).
-  eapply H.
-  descend; eauto.
-  rewrite H1; eauto.
-  eapply empty_mapsto_iff in H2; intuition.
+  subst; simpl in *.
+  contradict e.
+  Lemma Some_not_None : forall A o (v : A), o = Some v -> o <> None.
+    intuition.
+  Qed.
+  eapply Some_not_None.
+  eapply H0.
+  descend.
+  eauto.
+  left.
+  unfold gm, to_good_module in *; simpl in *.
+  descend.
+  eauto.
+  eauto.
+  simpl; eauto.
+  eauto.
+  simpl; eauto.
+  eapply empty_mapsto_iff in H3; intuition.
 Qed.
 
-Lemma stn_good : forall stn, stn_good_to_use modules imports stn -> from_bedrock_label_map (Labels stn) ("fact", "fact") <> None.
-  intros.
-  eapply H.
-  left; descend.
-  left; eauto.
-  unfold gm, to_good_module; simpl; eauto.
-  unfold gm, to_good_module; simpl; eauto.
-Qed.
-
-Lemma vcs_good : forall stn fs, stn_good_to_use modules imports stn -> fs_good_to_use' specs fs stn -> and_all (vc body empty_precond) (from_bedrock_label_map (Labels stn), fs stn).
+Lemma vcs_good : and_all (vc body empty_precond) specs.
   Ltac cito_vcs body := unfold body; simpl;
-    unfold imply_close, and_lift, interp; simpl(* ; *)
-      (* firstorder cito'; auto *).
+    unfold imply_close, and_lift, interp; simpl.
 
-  Ltac inversion_RunsTo :=
-    change ProgramLogicMake.SemanticsMake.RunsTo with RunsTo in *;
-    match goal with
-      | H : RunsTo _ _ _ _ |- _ => inversion H; unfold_all; subst;simpl in *; clear H
-    end.
+  Import ProgramLogicMake.SemanticsMake.
 
-  Ltac cito' :=
-    repeat (subst; simpl; selify; autorewrite with sepFormula in *; repeat inversion_RunsTo;
-      repeat match goal with
-               | [ H : _ |- _ ] => rewrite H
-             end).
+  Ltac destruct_state :=
+    repeat match goal with
+             | [ x : State |- _ ] => destruct x; simpl in *
+           end.
 
   unfold empty_precond.
 
   cito_vcs body.
-  intros; descend; intros; openhyp.
-  cito'.
-  econstructor; simpl.
-  eapply stn_good; eauto.
 
+  split.
+  intros.
+  openhyp.
   subst.
-  inversion H2; unfold_all; subst; simpl in *; clear H2.
-  unfold from_bedrock_label_map in *.
-
-  eapply SafeCallForeign; simpl in *.
+  unfold SafeDCall.
+  simpl.
+  intros.
+  destruct_state.
+  unfold TransitSafe.
+  descend.
   sel_upd_simpl.
-  eapply H0.
-  descend; eauto.
-  unfold specs; simpl.
-  reflexivity.
-
-  sel_upd_simpl.
-  instantiate (1 := [[ (sel (fst x) "n" ^- $1, inl (sel (fst x) "n" ^- $1)) ]]).
+  instantiate (1 := [[ (sel v "n" ^- $1, inl (sel v "n" ^- $1)) ]]).
   eauto.
   repeat constructor.
-  unfold PreCond; simpl.
   descend; eauto.
 
   eauto.
@@ -270,68 +250,51 @@ Qed.
 
 Local Hint Resolve final.
 
-Lemma body_runsto' : forall stn fs v v', stn_good_to_use modules imports stn -> fs_good_to_use' specs fs stn -> RunsTo (from_bedrock_label_map (Labels stn), fs stn) (Body f) v v' -> sel (fst v') (RetVar f) = fact_w (sel (fst v) "n") /\ snd v' = snd v.
-  unfold modules, imports.
-
-  Ltac cito_runsto f pre := intros;
-    match goal with
-      | [ H : _ |- _ ] => unfold f, Body, Core in H;
-        eapply sound_runsto' with (p := pre) (s := Body f) in H;
-          simpl in *; try eapply vcs_good; simpl in *;
-            auto; openhyp; subst; simpl in *; (* intuition auto;  *)unfold empty_precond, and_lift, or_lift in *; openhyp; [ .. | eauto ]
-    end.
-
-  cito_runsto f empty_precond.
+Lemma body_runsto' : forall env v v', specs_env_agree specs env -> RunsTo env (Body f) v v' -> sel (fst v') (RetVar f) = fact_w (sel (fst v) "n") /\ snd v' = snd v.
+  cito_runsto f empty_precond vcs_good.
+  3 : eauto.
   Focus 2.
-  cito'; eauto.
+  subst; simpl in *; eauto.
 
-  subst.
-  inversion H4; unfold_all; subst; simpl in *; clear H4.
-  unfold from_bedrock_label_map in *.
-
-  assert (fs0 stn w = Some (Foreign fact_spec)).
-  eapply H0.
-  descend.
-  eauto.
-  unfold specs; simpl.
-  reflexivity.
-
-  inversion H3; unfold_all; subst; simpl in *; clear H3.
-  sel_upd_simpl; rewrite H1 in H8; discriminate.
-  sel_upd_simpl; rewrite H1 in H8; injection H8; intros; subst.
-
+  subst; simpl in *.
+  sel_upd_simpl.
+  destruct_state.
+  unfold RunsToDCall in *.
+  simpl in *.
+  openhyp.
+  unfold TransitTo in *.
+  openhyp.
   unfold PostCond in *; simpl in *.
   openhyp.
   subst; simpl in *.
-  eapply triples_intro in H3; try eassumption.
+  eapply triples_intro in H5; try eassumption.
   subst; simpl in *.
-  Import Semantics.
-  unfold good_inputs in *.
+  unfold store_out, Semantics.store_out in *; simpl in *.
+  unfold good_inputs, Semantics.good_inputs in *.
   openhyp.
-  unfold word_adt_match in *.
+  unfold Semantics.word_adt_match in *.
   inversion_Forall; simpl in *.
-  subst.
-  unfold store_out in *; simpl in *.
-
-  inversion H2; unfold_all; subst; simpl in *; clear H2.
+  subst; simpl in *.
   sel_upd_simpl.
   split.
   symmetry; eapply fact_step; eauto.
+  eapply lt0_true in H3.
   eauto.
-
+  eauto.
+  
 Qed.
 
-Lemma body_safe' : forall stn fs v, stn_good_to_use modules imports stn -> fs_good_to_use' specs fs stn -> Safe (from_bedrock_label_map (Labels stn), fs stn) (Body f) v.
-  unfold modules, imports.
-  cito_safe f body empty_precond.
+Lemma body_safe' : forall env v, specs_env_agree specs env -> Safe env (Body f) v.
+  cito_safe f empty_precond vcs_good.
 Qed.
+
+Require LinkSpecFacts.
+Module LinkSpecFactsMake := LinkSpecFacts.Make ExampleADT.
 
 Lemma change_fs_strengthen : forall fs stn, stn_good_to_use modules imports stn -> fs_good_to_use modules imports fs stn ->strengthen (from_bedrock_label_map (Labels stn), fs stn) (from_bedrock_label_map (Labels stn), change_fs fs stn).
   unfold modules, imports.
   intros.
   generalize H0; intro.
-  eapply fs_good in H0.
-  unfold fs_good_to_use' in *.
   unfold strengthen.
   split.
   eauto.
@@ -341,25 +304,28 @@ Lemma change_fs_strengthen : forall fs stn, stn_good_to_use modules imports stn 
   intros.
   destruct (option_dec (fs0 stn w)); simpl in *.
   destruct s; rewrite e in *; simpl in *.
+  destruct x; simpl in *.
+  eauto.
   eapply H0 in e.
   openhyp.
-  unfold specs_op in H3.
-  eapply find_mapsto_iff in H3.
-  eapply add_mapsto_iff in H3.
+  subst; simpl in *.
   openhyp.
-  subst.
+  subst; simpl in *.
+  openhyp.
+  subst; simpl in *.
+  injection H3; intros; subst; simpl in *; clear H3.
   right; descend.
   eauto.
   eauto.
-  descend.
-  unfold PreCond in *; simpl in *.
+  simpl in *.
   openhyp.
+  descend.
   erewrite map_length_eq; eauto.
   eauto.
   eapply body_safe'; eauto.
-  eapply change_fs_good; eauto.
+  eapply change_fs_agree; eauto.
   eapply body_runsto' in H3; eauto.
-  2 : eapply change_fs_good; eauto.
+  2 : eapply change_fs_agree; eauto.
   openhyp.
   descend.
   instantiate (1 := [[ {| Word := sel (fst v) "n"; ADTIn := inl (sel (fst v) "n"); ADTOut := None |} ]]).
@@ -374,7 +340,9 @@ Lemma change_fs_strengthen : forall fs stn, stn_good_to_use modules imports stn 
   unfold f in *; simpl in *.
   rewrite H3.
   eauto.
-  eapply empty_mapsto_iff in H4; intuition.
+  intuition.
+  intuition.
+  rewrite empty_o in H4; intuition.
   rewrite e in *.
   eauto.
   Grab Existential Variables.
@@ -385,7 +353,7 @@ Lemma body_runsto : forall stn fs v v', stn_good_to_use modules imports stn -> f
   intros.
   eapply strengthen_runsto with (env_ax := (from_bedrock_label_map (Labels stn), change_fs fs0 stn)) in H1.
   eapply body_runsto'; eauto.
-  eapply change_fs_good; eauto.
+  eapply change_fs_agree; eauto.
   eapply change_fs_strengthen; eauto.
 Qed.
 
@@ -393,7 +361,7 @@ Lemma body_safe : forall stn fs v, stn_good_to_use modules imports stn -> fs_goo
   intros.
   eapply strengthen_safe.
   eapply body_safe'; eauto.
-  eapply change_fs_good; eauto.
+  eapply change_fs_agree; eauto.
   eapply change_fs_strengthen; eauto.
 Qed.
 
@@ -454,7 +422,7 @@ Theorem top_ok : moduleOk top.
   sep_auto.
 Qed.
 
-Definition all := link top (link_with_adts (gm :: nil) (empty _)).
+Definition all := link top (link_with_adts modules imports).
 
 Theorem all_ok : moduleOk all.
   link0 top_ok.
