platform/cito/LinkSpecFacts.v
@@ -1,0 +1,82 @@
+Set Implicit Arguments.
+
+Require Import ADT.
+
+Module Make (Import E : ADT).
+
+  Require Import LinkSpec.
+  Module Import LinkSpecMake := Make E.
+  Require Import ProgramLogic2.
+  Module Import ProgramLogicMake := Make E.
+
+  Section TopSection.
+
+    Notation FName := SyntaxFunc.Name.
+    Notation MName := GoodModule.Name.
+
+    Definition imports_exports_mapsto lbl spec modules imports :=
+      (exists ispec m f,
+         spec = Internal ispec /\
+         List.In m modules /\
+         List.In f (Functions m) /\
+         ispec = f /\ 
+         lbl = (MName m, FName f)) \/
+      (exists fspec,
+         spec = Foreign fspec /\
+         find lbl imports = Some fspec).
+
+    Definition imports_exports_in lbl modules (imports : t ForeignFuncSpec) :=
+      (exists m f,
+         List.In m modules /\
+         List.In f (Functions m) /\
+         lbl = (MName m, FName f)) \/
+      In lbl imports.
+
+    Require Import GeneralTactics.
+
+    Lemma imports_exports_mapsto_in : forall modules imports lbl spec, imports_exports_mapsto lbl spec modules imports -> imports_exports_in lbl modules imports.
+      unfold imports_exports_mapsto, imports_exports_in.
+      intros.
+      openhyp.
+      left; descend; eauto.
+      right; eapply MapsTo_In; eapply find_mapsto_iff; eauto.
+    Qed.
+
+    Definition specs_equal specs modules imports := forall lbl spec, find lbl specs = Some spec <-> imports_exports_mapsto lbl spec modules imports.
+
+    Lemma specs_equal_agree : forall specs modules imports, specs_equal specs modules imports -> forall stn fs, stn_good_to_use modules imports stn -> fs_good_to_use modules imports fs stn -> specs_env_agree specs (from_bedrock_label_map (Labels stn), fs stn).
+      intros.
+      split.
+
+      unfold labels_in_scope.
+      intros.
+      unfold from_bedrock_label_map in *; simpl in *.
+      eapply In_MapsTo in H2.
+      openhyp.
+      eapply H0.
+      eapply imports_exports_mapsto_in.
+      eapply H.
+      eapply find_mapsto_iff; eauto.
+
+      unfold specs_fs_agree.
+      unfold from_bedrock_label_map in *; simpl in *.
+      split; intros.
+
+      eapply H1 in H2.
+      destruct H2.
+      destruct H2.
+      descend.
+      eauto.
+      eapply H; eauto.
+
+      openhyp.
+      eapply H1.
+      eexists.
+      split.
+      eauto.
+      eapply H; eauto.
+    Qed.
+
+  End TopSection.
+
+End Make.
